an example of basic postprocessing of High code to Low, but also a failing tactic because of some unification trouble

examples/refinement/Example1.fst
@@ -30,59 +30,76 @@ let test =
     assert (LowComp.morph #_ _ (H.return_elab true) == L.lreturn true)
         by (dump "A"; apply_lemma (`L.morph_return); dump "B") //spawns SMT proof of monotonicity
 
+let heq_intro (#a:Type) (#b:Type) (x:a) (y:b) : Lemma (requires (a==b /\ x==y)) (ensures (x===y)) = ()
+
+let rewrite_morph lem () =
+  apply_lemma lem;
+  dismiss();
+  apply_lemma (`heq_intro);
+  split(); flip();
+  trefl(); trefl()
+
+[@(postprocess_with (rewrite_morph (`L.morph_return)))]
+let test_rewrite = morph (H.return_elab true)
+
 let test2 =
     assert (LowComp.morph #_ _ (H.hread_elab 0) == L.lread' 0)
         by (apply_lemma (`L.morph_read))
 
+[@(postprocess_with (rewrite_morph (`L.morph_read)))]
+let test2' = morph (H.hread_elab 0)
+
 let test3 (#a:Type0) (#b:Type0)
           (#wpa:H.hwp_mon a) (#wpb: (a -> H.hwp_mon b))
           (c1:H.comp_wp a wpa) (c2: (x:a -> H.comp_wp b (wpb x))) =
-    assert (LowComp.morph #_ _ (H.bind_elab c1 c2) == L.lbind (morph c1) (fun x -> morph (c2 x)))
+    assert (morph (H.bind_elab c1 c2) == L.lbind (morph c1) (fun x -> morph (c2 x)))
         by (apply_lemma (`L.morph_bind))
 
+//Needs a use of fext, rightfully so
+[@(expect_failure)
+  (postprocess_with (rewrite_morph (`L.morph_bind)))]
+let test3' (#a:Type0) (#b:Type0)
+           (#wpa:H.hwp_mon a) (#wpb: (a -> H.hwp_mon b))
+           (c1:H.comp_wp a wpa) (c2: (x:a -> H.comp_wp b (wpb x))) =
+    morph (H.bind_elab c1 c2)
+
 open FStar.FunctionalExtensionality
-
-
-let apply_feq2_lem #a #b #c ($f $g : a -> b -> c) : Lemma (requires (forall x y. f x y == g x y))
-                                                        (ensures (f == g)) =
-    assert (forall x. feq (f x) (g x));
-    assert (feq f g)
-
-
 let apply_feq_lem #a #b ($f $g : a -> b) : Lemma (requires (forall x. f x == g x))
                                                 (ensures (f == g)) =
     assert (feq f g)
 
 let fext () = apply_lemma (`apply_feq_lem); dismiss (); ignore (forall_intros ())
 
-let morph_bind () = dump "A"; fext (); dump "B"; apply_lemma (`L.morph_bind)
-
-#set-options "--debug Example1 --debug_level Rel"
-//[@(postprocess_with morph_bind)]
-let test4 (#a:Type0)
+//TODO: But uses of fext fail on this occurrence below (some unification trouble?)
+[@(expect_failure)]
+let test_feq
+          (#a:Type0)
           (#b:Type0)
           (#wpa:H.hwp_mon a)
           (#wpb: (a -> H.hwp_mon b))
           (c1:H.comp_wp a wpa)
-           =
-    assert ((fun (c2: (x:a -> H.comp_wp b (wpb x))) ->
-              LowComp.morph #b (H.bind_wp wpa wpb) (H.bind_elab c1 c2)) ==
-            (fun (c2: (x:a -> H.comp_wp b (wpb x))) -> L.lbind (morph c1) (fun x -> morph (c2 x))))
-       by (dump "A"; fext(); dump "B")
+          =
+  assert ((fun (c2:(x:a -> H.comp_wp b (wpb x))) ->
+             LowComp.morph #b (H.bind_wp wpa wpb) (H.bind_elab c1 c2)) ==
+          (fun (c2: (x:a -> H.comp_wp b (wpb x))) ->
+             L.lbind (morph c1) (fun x -> morph (c2 x))))
+      by (dump "Before";
+          apply_lemma (`apply_feq_lem);
+          dump "1";
+          ignore (forall_intros ());
+          dump "After";
+          tadmit())
 
-    // assert (morph (H.bind_elab c1 c2) === L.lbind (morph c1) (fun x -> morph (c2 x)))
-    //     by (apply_lemma (`L.morph_bind))
 
-// let swap : comp_wp unit _ =
-//   bind_elab (get_action 0) (fun x0 0
+//Ultimately, would like to write code like this
+let sum_and_swap () : Hi uint_32
+    (requires (fun (x0, x1) -> ok (+) x0 x1)) //precondition rules out overflow
+    (ensures (fun _ _ _ -> True)) =
+   let x0 = H.get_action 0 in
+   let x1 = H.get_action 1 in
+   H.put_action 0 x1;
+   H.put_action 1 x0;
+   x0 + x1
 
-// let sum_and_swap () : Hi uint_32
-//     (requires (fun (x0, x1) -> ok (+) x0 x1))
-//     (ensures (fun _ _ _ -> True)) =
-//    let x0 = H.get_action 0 in
-//    let x1 = H.get_action 1 in
-//    H.put_action 0 x1;
-//    H.put_action 1 x0;
-//    x0 + x1
-
-// // let test2 = morph (reify (sum_and_swap ()))
+[@(postprocess_with (fun () -> trefl()))] //using a rewrite tactic here
+let sum_and_swap_low () = morph (reify (sum_and_swap ()))
